`--z3_skip_c_initializers` to omit field labels
this option is needed for C++ compilers older than C++20

src/3d/Options.fst
@@ -50,7 +50,6 @@ let valid_micro_step (str: string) : Tot bool = match str with
   | "emit_config"
     -> true
   | _ -> false
-
 let micro_step : ref (option (valid_string valid_micro_step)) = alloc None
 
 let produce_c_from_existing_krml : ref bool = alloc false
@@ -120,6 +119,8 @@ let test_checker : ref (option vstring) = alloc None
 let z3_branch_depth : ref (option vstring) = alloc None
 
 let z3_options : ref (option vstring) = alloc None
+
+let z3_skip_c_initializers: ref bool = alloc false
 
 let char_le (c1 c2: FStar.Char.char) : Tot bool =
   FStar.Char.int_of_char c1 <= FStar.Char.int_of_char c2
@@ -378,6 +379,7 @@ let (display_usage_2, compute_options_2, fstar_options) =
     CmdOption "z3_executable" (OptStringOption "path/to/z3" always_valid z3_executable) "z3 executable for test case generation (default `z3`; does not affect verification of generated F* code)" [];
     CmdOption "z3_options" (OptStringOption "'options to z3'" always_valid z3_options) "command-line options to pass to z3 for test case generation (does not affect verification of generated F* code)" [];
     CmdOption "z3_skip_testcases_c" (OptBool no_produce_testcases_c) "skip generating test cases to <output directory>/testcases.c" [];
+    CmdOption "z3_skip_c_initializers" (OptBool z3_skip_c_initializers) "Do not use C field initializers for test cases" [];
     CmdOption "z3_test" (OptStringOption "parser name" always_valid z3_test) "produce positive and/or negative test cases for a given parser" [];
     CmdOption "z3_test_mode" (OptStringOption "pos|neg|all" valid_z3_test_mode z3_test_mode) "produce positive, negative, or all kinds of test cases (default all)" [];
     CmdOption "z3_witnesses" (OptStringOption "nb" always_valid z3_witnesses) "ask for nb distinct test witnesses per branch case (default 1)" [];
@@ -615,6 +617,9 @@ let get_z3_flight_name () : ML string =
 
 let get_produce_testcases_c () : ML bool =
   not !no_produce_testcases_c
+
+let get_z3_skip_c_initializers () : ML bool =
+  !z3_skip_c_initializers
 
 let get_fstar_exe () : ML string =
   match !fstar_exe with
