src/3d/Options.fsti
@@ -86,4 +86,6 @@ val get_z3_flight_name: unit -> ML string
 
 val get_produce_testcases_c: unit -> ML bool
 
+val get_z3_skip_c_initializers: unit -> ML bool
+
 val get_fstar_exe: unit -> ML string
